------------------------------------------------------------------------------
-- Elimination properties for the inequalities
------------------------------------------------------------------------------

{-# OPTIONS --exact-split              #-}
{-# OPTIONS --no-sized-types           #-}
{-# OPTIONS --no-universe-polymorphism #-}
{-# OPTIONS --without-K                #-}

module Combined.FOTC.Data.Nat.Inequalities.EliminationProperties where

open import Combined.FOTC.Base
open import Combined.FOTC.Data.Nat
open import Combined.FOTC.Data.Nat.Inequalities

------------------------------------------------------------------------------

0<0→⊥ : ¬ (zero < zero)
0<0→⊥ h = prf
  where postulate prf : ⊥
        {-# ATP prove prf #-}

x<0→⊥ : ∀ {n} → N n → ¬ (n < zero)
x<0→⊥ nzero h = prf
  where postulate prf : ⊥
        {-# ATP prove prf #-}
x<0→⊥ (nsucc Nn) h = prf
  where postulate prf : ⊥
        {-# ATP prove prf #-}

x<x→⊥ : ∀ {n} → N n → ¬ (n < n)
x<x→⊥ nzero h = prf
  where postulate prf : ⊥
        {-# ATP prove prf #-}
x<x→⊥ (nsucc {n} Nn) h = prf (x<x→⊥ Nn)
  where postulate prf : ¬ (n < n) → ⊥
        {-# ATP prove prf #-}

0>x→⊥ : ∀ {n} → N n → ¬ (zero > n)
0>x→⊥ nzero h = prf
  where postulate prf : ⊥
        {-# ATP prove prf #-}
0>x→⊥ (nsucc Nn) h = prf
  where postulate prf : ⊥
        {-# ATP prove prf #-}

S≤0→⊥ : ∀ {n} → N n → ¬ (succ₁ n ≤ zero)
S≤0→⊥ nzero h = prf
  where postulate prf : ⊥
        {-# ATP prove prf #-}
S≤0→⊥ (nsucc {n} Nn) h = prf
  where postulate prf : ⊥
        {-# ATP prove prf #-}

0≥S→⊥ : ∀ {n} → N n → ¬ (zero ≥ succ₁ n)
0≥S→⊥ Nn h = prf
  where postulate prf : ⊥
        {-# ATP prove prf S≤0→⊥ #-}

postulate S≯0→⊥ : ∀ {n} → ¬ (succ₁ n ≯ zero)
{-# ATP prove S≯0→⊥ #-}

x<y→y<x→⊥ : ∀ {m n} → N m → N n → m < n → ¬ (n < m)
x<y→y<x→⊥ nzero Nn h₁ h₂ = prf
  where postulate prf : ⊥
        {-# ATP prove prf 0>x→⊥ #-}
x<y→y<x→⊥ (nsucc Nm) nzero h₁ h₂ = prf
  where postulate prf : ⊥
        {-# ATP prove prf 0>x→⊥ #-}
x<y→y<x→⊥ (nsucc {m} Nm) (nsucc {n} Nn) h₁ h₂ = prf (x<y→y<x→⊥ Nm Nn m<n)
  where
  postulate m<n : m < n
  {-# ATP prove m<n #-}

  postulate prf : ¬ (n < m) → ⊥
  {-# ATP prove prf #-}

x>y→x≤y→⊥ : ∀ {m n} → N m → N n → m > n → ¬ (m ≤ n)
x>y→x≤y→⊥ nzero Nn h₁ h₂ = prf
  where postulate prf : ⊥
        {-# ATP prove prf x<0→⊥ #-}
x>y→x≤y→⊥ (nsucc Nm) nzero h₁ h₂ = prf
  where postulate prf : ⊥
        {-# ATP prove prf x<0→⊥ #-}
x>y→x≤y→⊥ (nsucc {m} Nm) (nsucc {n} Nn) h₁ h₂ = prf (x>y→x≤y→⊥ Nm Nn m>n)
  where
  postulate m>n : m > n
  {-# ATP prove m>n #-}

  postulate prf : ¬ (m ≤ n) → ⊥
  {-# ATP prove prf #-}
