------------------------------------------------------------------------------
-- The gcd is divisible by any common divisor
------------------------------------------------------------------------------

{-# OPTIONS --exact-split              #-}
{-# OPTIONS --no-sized-types           #-}
{-# OPTIONS --no-universe-polymorphism #-}
{-# OPTIONS --without-K                #-}

module Combined.FOTC.Program.GCD.Total.Divisible where

open import Combined.FOTC.Base
open import Combined.FOTC.Data.Nat
open import Combined.FOTC.Data.Nat.Divisibility.By0
open import Combined.FOTC.Data.Nat.Divisibility.By0.Properties
open import Combined.FOTC.Data.Nat.Induction.NonAcc.Lexicographic
open import Combined.FOTC.Data.Nat.Inequalities
open import Combined.FOTC.Data.Nat.Inequalities.EliminationProperties
open import Combined.FOTC.Data.Nat.Inequalities.Properties
open import Combined.FOTC.Data.Nat.Properties
open import Combined.FOTC.Program.GCD.Total.Definitions
open import Combined.FOTC.Program.GCD.Total.GCD

------------------------------------------------------------------------------
-- The gcd 0 0 is Divisible.
postulate gcd-00-Divisible : Divisible zero zero (gcd zero zero)
{-# ATP prove gcd-00-Divisible #-}

-- The gcd 0 (succ n) is Divisible.
postulate
  gcd-0S-Divisible : ∀ {n} → N n → Divisible zero (succ₁ n) (gcd zero (succ₁ n))
{-# ATP prove gcd-0S-Divisible #-}

postulate
  gcd-S0-Divisible : ∀ {n} → N n → Divisible (succ₁ n) zero (gcd (succ₁ n) zero)
{-# ATP prove gcd-S0-Divisible #-}

------------------------------------------------------------------------------
-- The gcd (succ₁ m) (succ₁ n) when succ₁ m > succ₁ n is Divisible.
-- For the proof using the ATP we added the helper hypothesis
-- c | succ₁ m → c | succ₁ c → c | succ₁ m ∸ succ₁ n.
postulate
  gcd-S>S-Divisible-ah :
    ∀ {m n} → N m → N n →
    (Divisible (succ₁ m ∸ succ₁ n) (succ₁ n) (gcd (succ₁ m ∸ succ₁ n) (succ₁ n))) →
    succ₁ m > succ₁ n →
    ∀ c → N c → CD (succ₁ m) (succ₁ n) c →
    (c ∣ succ₁ m ∸ succ₁ n) →
    c ∣ gcd (succ₁ m) (succ₁ n)
{-# ATP prove gcd-S>S-Divisible-ah #-}

gcd-S>S-Divisible :
  ∀ {m n} → N m → N n →
  (Divisible (succ₁ m ∸ succ₁ n) (succ₁ n) (gcd (succ₁ m ∸ succ₁ n) (succ₁ n))) →
  succ₁ m > succ₁ n →
  Divisible (succ₁ m) (succ₁ n) (gcd (succ₁ m) (succ₁ n))
gcd-S>S-Divisible {m} {n} Nm Nn acc Sm>Sn c Nc (c∣Sm , c∣Sn) =
    gcd-S>S-Divisible-ah Nm Nn acc Sm>Sn c Nc (c∣Sm , c∣Sn)
                         (x∣y→x∣z→x∣y∸z Nc (nsucc Nm) (nsucc Nn) c∣Sm c∣Sn)

------------------------------------------------------------------------------
-- The gcd (succ₁ m) (succ₁ n) when succ₁ m ≯ succ₁ n is Divisible.
-- For the proof using the ATP we added the helper hypothesis
-- c | succ₁ n → c | succ₁ m → c | succ₁ n ∸ succ₁ m.
postulate
  gcd-S≯S-Divisible-ah :
    ∀ {m n} → N m → N n →
    (Divisible (succ₁ m) (succ₁ n ∸ succ₁ m) (gcd (succ₁ m) (succ₁ n ∸ succ₁ m))) →
    succ₁ m ≯ succ₁ n →
    ∀ c → N c → CD (succ₁ m) (succ₁ n) c →
    (c ∣ succ₁ n ∸ succ₁ m) →
    c ∣ gcd (succ₁ m) (succ₁ n)
{-# ATP prove gcd-S≯S-Divisible-ah #-}

gcd-S≯S-Divisible :
  ∀ {m n} → N m → N n →
  (Divisible (succ₁ m) (succ₁ n ∸ succ₁ m) (gcd (succ₁ m) (succ₁ n ∸ succ₁ m))) →
  succ₁ m ≯ succ₁ n →
  Divisible (succ₁ m) (succ₁ n) (gcd (succ₁ m) (succ₁ n))
gcd-S≯S-Divisible {m} {n} Nm Nn acc Sm≯Sn c Nc (c∣Sm , c∣Sn) =
    gcd-S≯S-Divisible-ah Nm Nn acc Sm≯Sn c Nc (c∣Sm , c∣Sn)
                         (x∣y→x∣z→x∣y∸z Nc (nsucc Nn) (nsucc Nm) c∣Sn c∣Sm)

------------------------------------------------------------------------------
-- The gcd m n when m > n is Divisible.
gcd-x>y-Divisible :
  ∀ {m n} → N m → N n →
  (∀ {o p} → N o → N p → Lexi o p m n → Divisible o p (gcd o p)) →
  m > n →
  Divisible m n (gcd m n)
gcd-x>y-Divisible nzero Nn _ 0>n _ _ = ⊥-elim (0>x→⊥ Nn 0>n)
gcd-x>y-Divisible (nsucc Nm) nzero _ _ c Nc = gcd-S0-Divisible Nm c Nc
gcd-x>y-Divisible (nsucc {m} Nm) (nsucc {n} Nn) ah Sm>Sn c Nc =
  gcd-S>S-Divisible Nm Nn ih Sm>Sn c Nc
  where
  -- Inductive hypothesis.
  ih : Divisible (succ₁ m ∸ succ₁ n) (succ₁ n) (gcd (succ₁ m ∸ succ₁ n) (succ₁ n))
  ih = ah {succ₁ m ∸ succ₁ n}
          {succ₁ n}
          (∸-N (nsucc Nm) (nsucc Nn))
          (nsucc Nn)
          ([Sx∸Sy,Sy]<[Sx,Sy] Nm Nn)

------------------------------------------------------------------------------
-- The gcd m n when m ≯ n is Divisible.
gcd-x≯y-Divisible :
  ∀ {m n} → N m → N n →
  (∀ {o p} → N o → N p → Lexi o p m n → Divisible o p (gcd o p)) →
  m ≯ n →
  Divisible m n (gcd m n)
gcd-x≯y-Divisible nzero nzero _ _ c Nc = gcd-00-Divisible c Nc
gcd-x≯y-Divisible nzero (nsucc Nn) _ _ c Nc = gcd-0S-Divisible Nn c Nc
gcd-x≯y-Divisible (nsucc _) nzero _ Sm≯0 _ _ = ⊥-elim (S≯0→⊥ Sm≯0)
gcd-x≯y-Divisible (nsucc {m} Nm) (nsucc {n} Nn) ah Sm≯Sn c Nc =
  gcd-S≯S-Divisible Nm Nn ih Sm≯Sn c Nc
  where
  -- Inductive hypothesis.
  ih : Divisible (succ₁ m) (succ₁ n ∸ succ₁ m) (gcd (succ₁ m) (succ₁ n ∸ succ₁ m))
  ih = ah {succ₁ m}
          {succ₁ n ∸ succ₁ m}
          (nsucc Nm)
          (∸-N (nsucc Nn) (nsucc Nm))
          ([Sx,Sy∸Sx]<[Sx,Sy] Nm Nn)

------------------------------------------------------------------------------
-- The gcd is Divisible.
gcdDivisible : ∀ {m n} → N m → N n → Divisible m n (gcd m n)
gcdDivisible = Lexi-wfind A h
  where
  A : D → D → Set
  A i j = Divisible i j (gcd i j)

  h : ∀ {i j} → N i → N j → (∀ {k l} → N k → N l → Lexi k l i j → A k l) →
      A i j
  h Ni Nj ah = case (gcd-x>y-Divisible Ni Nj ah)
                    (gcd-x≯y-Divisible Ni Nj ah)
                    (x>y∨x≯y Ni Nj)
