------------------------------------------------------------------------------
-- The gcd is commutative
------------------------------------------------------------------------------

{-# OPTIONS --exact-split              #-}
{-# OPTIONS --no-sized-types           #-}
{-# OPTIONS --no-universe-polymorphism #-}
{-# OPTIONS --without-K                #-}

module InteractiveFOT.FOTC.Program.GCD.Total.Commutative where

open import Common.FOL.Relation.Binary.EqReasoning

open import Interactive.FOTC.Base
open import Interactive.FOTC.Data.Nat
open import Interactive.FOTC.Data.Nat.Induction.NonAcc.Lexicographic
open import Interactive.FOTC.Data.Nat.Inequalities
open import Interactive.FOTC.Data.Nat.Inequalities.EliminationProperties
open import Interactive.FOTC.Data.Nat.Inequalities.Properties
open import Interactive.FOTC.Data.Nat.Properties
open import Interactive.FOTC.Program.GCD.Total.ConversionRules
open import Interactive.FOTC.Program.GCD.Total.GCD

------------------------------------------------------------------------------
-- Informal proof:
-- 1. gcd 0 n = n        -- gcd def
--            = gcd n 0  -- gcd def

-- 2. gcd n 0 = n        -- gcd def
--            = gcd 0 n  -- gcd def

-- 3.1. Case: S m > S n
-- gcd (S m) (S n) = gcd (S m - S n) (S n)  -- gcd def
--                 = gcd (S n) (S m - S n)  -- IH
--                 = gcd (S n) (S m)        -- gcd def

-- 3.2. Case: S m ≮ S n
-- gcd (S m) (S n) = gcd (S m) (S n - S m)  -- gcd def
--                 = gcd (S n - S m) (S m)  -- IH
--                 = gcd (S n) (S m)        -- gcd def

------------------------------------------------------------------------------
-- Commutativity property.
Comm : D → D → Set
Comm t t' = gcd t t' ≡ gcd t' t

x>y→y≯x : ∀ {m n} → N m → N n → m > n → n ≯ m
x>y→y≯x nzero          Nn             0>n   = ⊥-elim (0>x→⊥ Nn 0>n)
{-# CATCHALL #-}
x>y→y≯x Nm             nzero          _     = 0≯x Nm
x>y→y≯x (nsucc {m} Nm) (nsucc {n} Nn) Sm>Sn =
  trans (lt-SS m n) (x>y→y≯x Nm Nn (trans (sym (lt-SS n m)) Sm>Sn))

postulate x≯Sy→Sy>x : ∀ {m n} → N m → N n → m ≯ succ₁ n → succ₁ n > m
-- x≯Sy→Sy>x {n = n} nzero      Nn _ = <-0S n
-- x≯Sy→Sy>x {n = n} (nsucc {m} Nm) Nn h = {!!}

------------------------------------------------------------------------------
-- gcd 0 0 is commutative.
gcd-00-comm : Comm zero zero
gcd-00-comm = refl

------------------------------------------------------------------------------
-- gcd (succ₁ n) 0 is commutative.
gcd-S0-comm : ∀ n → Comm (succ₁ n) zero
gcd-S0-comm n = trans (gcd-S0 n) (sym (gcd-0S n))

------------------------------------------------------------------------------
-- gcd (succ₁ m) (succ₁ n) when succ₁ m > succ₁ n is commutative.
gcd-S>S-comm : ∀ {m n} → N m → N n →
               Comm (succ₁ m ∸ succ₁ n) (succ₁ n) →
               succ₁ m > succ₁ n →
               Comm (succ₁ m) (succ₁ n)
gcd-S>S-comm {m} {n} Nm Nn ih Sm>Sn =
  gcd (succ₁ m) (succ₁ n)
    ≡⟨ gcd-S>S m n Sm>Sn ⟩
  gcd (succ₁ m ∸ succ₁ n) (succ₁ n)
    ≡⟨ ih ⟩
  gcd (succ₁ n) (succ₁ m ∸ succ₁ n)
    ≡⟨ sym (gcd-S≯S n m (x>y→y≯x (nsucc Nm) (nsucc Nn) Sm>Sn)) ⟩
  gcd (succ₁ n) (succ₁ m) ∎

------------------------------------------------------------------------------
-- gcd (succ₁ m) (succ₁ n) when succ₁ m ≯ succ₁ n is commutative.
gcd-S≯S-comm : ∀ {m n} → N m → N n →
               Comm (succ₁ m) (succ₁ n ∸ succ₁ m) →
               succ₁ m ≯ succ₁ n →
               Comm (succ₁ m) (succ₁ n)
gcd-S≯S-comm {m} {n} Nm Nn ih Sm≯Sn =
  gcd (succ₁ m) (succ₁ n)
    ≡⟨ gcd-S≯S m n Sm≯Sn ⟩
  gcd (succ₁ m) (succ₁ n ∸ succ₁ m)
    ≡⟨ ih ⟩
  gcd (succ₁ n ∸ succ₁ m) (succ₁ m)
    ≡⟨ sym (gcd-S>S n m (x≯Sy→Sy>x (nsucc Nm) Nn Sm≯Sn)) ⟩
  gcd (succ₁ n) (succ₁ m) ∎

------------------------------------------------------------------------------
-- gcd m n when m > n is commutative.
gcd-x>y-comm :
  ∀ {m n} → N m → N n →
  (∀ {o p} → N o → N p → Lexi o p m n → Comm o p) →
  m > n →
  Comm m n
gcd-x>y-comm nzero          Nn             _  0>n   = ⊥-elim (0>x→⊥ Nn 0>n)
gcd-x>y-comm (nsucc {n} _)  nzero          _  _     = gcd-S0-comm n
gcd-x>y-comm (nsucc {m} Nm) (nsucc {n} Nn) ah Sm>Sn = gcd-S>S-comm Nm Nn ih Sm>Sn
  where
  -- Inductive hypothesis.
  ih : Comm (succ₁ m ∸ succ₁ n) (succ₁ n)
  ih = ah {succ₁ m ∸ succ₁ n}
          {succ₁ n}
          (∸-N (nsucc Nm) (nsucc Nn))
          (nsucc Nn)
          ([Sx∸Sy,Sy]<[Sx,Sy] Nm Nn)

------------------------------------------------------------------------------
-- gcd m n when m ≯ n is commutative.
gcd-x≯y-comm :
  ∀ {m n} → N m → N n →
  (∀ {o p} → N o → N p → Lexi o p m n → Comm o p) →
  m ≯ n →
  Comm m n
gcd-x≯y-comm nzero          nzero          _  _     = gcd-00-comm
gcd-x≯y-comm nzero          (nsucc {n} _)  _  _     = sym (gcd-S0-comm n)
gcd-x≯y-comm (nsucc _)      nzero          _  Sm≯0  = ⊥-elim (S≯0→⊥ Sm≯0)
gcd-x≯y-comm (nsucc {m} Nm) (nsucc {n} Nn) ah Sm≯Sn = gcd-S≯S-comm Nm Nn ih Sm≯Sn
  where
  -- Inductive hypothesis.
  ih : Comm (succ₁ m) (succ₁ n ∸ succ₁ m)
  ih = ah {succ₁ m}
          {succ₁ n ∸ succ₁ m}
          (nsucc Nm)
          (∸-N (nsucc Nn) (nsucc Nm))
          ([Sx,Sy∸Sx]<[Sx,Sy] Nm Nn)

------------------------------------------------------------------------------
-- gcd is commutative.
gcd-comm : ∀ {m n} → N m → N n → Comm m n
gcd-comm = Lexi-wfind A h
  where
  A : D → D → Set
  A i j = Comm i j

  h : ∀ {i j} → N i → N j → (∀ {k l} → N k → N l → Lexi k l i j → A k l) →
      A i j
  h Ni Nj ah = case (gcd-x>y-comm Ni Nj ah)
                    (gcd-x≯y-comm Ni Nj ah)
                    (x>y∨x≯y Ni Nj)
