------------------------------------------------------------------------------
-- The gcd is a common divisor
------------------------------------------------------------------------------

{-# OPTIONS --exact-split              #-}
{-# OPTIONS --no-sized-types           #-}
{-# OPTIONS --no-universe-polymorphism #-}
{-# OPTIONS --without-K                #-}

module Combined.FOTC.Program.GCD.Partial.CommonDivisor where

open import Combined.FOTC.Base
open import Combined.FOTC.Base.Properties
open import Combined.FOTC.Data.Nat
open import Combined.FOTC.Data.Nat.Divisibility.NotBy0
open import Combined.FOTC.Data.Nat.Divisibility.NotBy0.Properties
open import Combined.FOTC.Data.Nat.Induction.NonAcc.Lexicographic
open import Combined.FOTC.Data.Nat.Inequalities
open import Combined.FOTC.Data.Nat.Inequalities.EliminationProperties
open import Combined.FOTC.Data.Nat.Inequalities.Properties
open import Combined.FOTC.Data.Nat.Properties
open import Combined.FOTC.Program.GCD.Partial.Definitions
open import Combined.FOTC.Program.GCD.Partial.GCD
open import Combined.FOTC.Program.GCD.Partial.Totality

------------------------------------------------------------------------------
-- Some cases of the gcd-∣₁.

-- We don't prove that
--
-- gcd-∣₁ : ... → (gcd m n) ∣ m

-- because this proof should be defined mutually recursive with the
-- proof
--
-- gcd-∣₂ : ... → (gcd m n) ∣ n.
--
-- Therefore, instead of proving
--
-- gcdCD : ... → CD m n (gcd m n)
--
-- using these proofs (i.e. the conjunction of them), we proved it
-- using well-founded induction.

-- gcd 0 (succ n) ∣ 0.
postulate gcd-0S-∣₁ : ∀ {n} → N n → gcd zero (succ₁ n) ∣ zero
{-# ATP prove gcd-0S-∣₁ #-}

-- gcd (succ₁ m) 0 ∣ succ₁ m.
postulate gcd-S0-∣₁ : ∀ {n} → N n → gcd (succ₁ n) zero ∣ succ₁ n
{-# ATP prove gcd-S0-∣₁ ∣-refl-S #-}

-- gcd (succ₁ m) (succ₁ n) ∣ succ₁ m, when succ₁ m ≯ succ₁ n.
postulate gcd-S≯S-∣₁ : ∀ {m n} → N m → N n →
                       (gcd (succ₁ m) (succ₁ n ∸ succ₁ m) ∣ succ₁ m) →
                       succ₁ m ≯ succ₁ n →
                       gcd (succ₁ m) (succ₁ n) ∣ succ₁ m
{-# ATP prove gcd-S≯S-∣₁ #-}

-- gcd (succ₁ m) (succ₁ n) ∣ succ₁ m when succ₁ m > succ₁ n.
{- Proof:
1. gcd (Sm ∸ Sn) Sn | (Sm ∸ Sn)        IH
2. gcd (Sm ∸ Sn) Sn | Sn               gcd-∣₂
3. gcd (Sm ∸ Sn) Sn | (Sm ∸ Sn) + Sn   m∣n→m∣o→m∣n+o 1,2
4. Sm > Sn                             Hip
5. gcd (Sm ∸ Sn) Sn | Sm               arith-gcd-m>n₂ 3,4
6. gcd Sm Sn = gcd (Sm ∸ Sn) Sn        gcd eq. 4
7. gcd Sm Sn | Sm                      subst 5,6
-}

-- For the proof using the ATP we added the helper hypothesis:
-- 1. gcd (succ₁ m ∸ succ₁ n) (succ₁ n) ∣ (succ₁ m ∸ succ₁ n) + succ₁ n.
-- 2. (succ₁ m ∸ succ₁ n) + succ₁ n ≡ succ₁ m.
postulate
  gcd-S>S-∣₁-ah :
    ∀ {m n} → N m → N n →
    (gcd (succ₁ m ∸ succ₁ n) (succ₁ n) ∣ (succ₁ m ∸ succ₁ n)) →
    (gcd (succ₁ m ∸ succ₁ n) (succ₁ n) ∣ succ₁ n) →
    succ₁ m > succ₁ n →
    gcd (succ₁ m ∸ succ₁ n) (succ₁ n) ∣ (succ₁ m ∸ succ₁ n) + succ₁ n →
    ((succ₁ m ∸ succ₁ n) + succ₁ n ≡ succ₁ m) →
    gcd (succ₁ m) (succ₁ n) ∣ succ₁ m
{-# ATP prove gcd-S>S-∣₁-ah #-}

gcd-S>S-∣₁ :
  ∀ {m n} → N m → N n →
  (gcd (succ₁ m ∸ succ₁ n) (succ₁ n) ∣ (succ₁ m ∸ succ₁ n)) →
  (gcd (succ₁ m ∸ succ₁ n) (succ₁ n) ∣ succ₁ n) →
  succ₁ m > succ₁ n →
  gcd (succ₁ m) (succ₁ n) ∣ succ₁ m
gcd-S>S-∣₁ {m} {n} Nm Nn ih gcd-∣₂ Sm>Sn =
  gcd-S>S-∣₁-ah Nm Nn ih gcd-∣₂ Sm>Sn
    (x∣y→x∣z→x∣y+z gcd-Sm-Sn,Sn-N Sm-Sn-N (nsucc Nn) ih gcd-∣₂)
    (x>y→x∸y+y≡x (nsucc Nm) (nsucc Nn) Sm>Sn)

  where
  Sm-Sn-N : N (succ₁ m ∸ succ₁ n)
  Sm-Sn-N = ∸-N (nsucc Nm) (nsucc Nn)

  gcd-Sm-Sn,Sn-N : N (gcd (succ₁ m ∸ succ₁ n) (succ₁ n))
  gcd-Sm-Sn,Sn-N = gcd-N Sm-Sn-N (nsucc Nn) (λ p → ⊥-elim (S≢0 (∧-proj₂ p)))

------------------------------------------------------------------------------
-- Some case of the gcd-∣₂.
-- We don't prove that gcd-∣₂ : ... → gcd m n ∣ n. The reason is
-- the same to don't prove gcd-∣₁ : ... → gcd m n ∣ m.

-- gcd 0 (succ₁ n) ∣₂ succ₁ n.
postulate gcd-0S-∣₂ : ∀ {n} → N n → gcd zero (succ₁ n) ∣ succ₁ n
{-# ATP prove gcd-0S-∣₂ ∣-refl-S #-}

-- gcd (succ₁ m) 0 ∣ 0.
postulate gcd-S0-∣₂ : ∀ {m} → N m → gcd (succ₁ m) zero ∣ zero
{-# ATP prove gcd-S0-∣₂ #-}

-- gcd (succ₁ m) (succ₁ n) ∣ succ₁ n when succ₁ m ≯ succ₁ n.
{- Proof:
1. gcd Sm (Sn ∸ Sm) | (Sn ∸ Sm)        IH
2  gcd Sm (Sn ∸ Sm) | Sm               gcd-∣₁
3. gcd Sm (Sn ∸ Sm) | (Sn ∸ Sm) + Sm   m∣n→m∣o→m∣n+o 1,2
4. Sm ≯ Sn                             Hip
5. gcd (Sm ∸ Sn) Sn | Sm               arith-gcd-m≤n₂ 3,4
6. gcd Sm Sn = gcd Sm (Sn ∸ Sm)        gcd eq. 4
7. gcd Sm Sn | Sn                      subst 5,6
-}

-- For the proof using the ATP we added the helper hypothesis:
-- 1. gcd (succ₁ m) (succ₁ n ∸ succ₁ m) ∣ (succ₁ n ∸ succ₁ m) + succ₁ m.
-- 2 (succ₁ n ∸ succ₁ m) + succ₁ m ≡ succ₁ n.
postulate
  gcd-S≯S-∣₂-ah :
    ∀ {m n} → N m → N n →
    (gcd (succ₁ m) (succ₁ n ∸ succ₁ m) ∣ (succ₁ n ∸ succ₁ m)) →
    (gcd (succ₁ m) (succ₁ n ∸ succ₁ m) ∣ succ₁ m) →
    succ₁ m ≯ succ₁ n →
    (gcd (succ₁ m) (succ₁ n ∸ succ₁ m) ∣ (succ₁ n ∸ succ₁ m) + succ₁ m) →
    ((succ₁ n ∸ succ₁ m) + succ₁ m ≡ succ₁ n) →
    gcd (succ₁ m) (succ₁ n) ∣ succ₁ n
{-# ATP prove gcd-S≯S-∣₂-ah #-}

gcd-S≯S-∣₂ :
  ∀ {m n} → N m → N n →
  (gcd (succ₁ m) (succ₁ n ∸ succ₁ m) ∣ (succ₁ n ∸ succ₁ m)) →
  (gcd (succ₁ m) (succ₁ n ∸ succ₁ m) ∣ succ₁ m) →
  succ₁ m ≯ succ₁ n →
  gcd (succ₁ m) (succ₁ n) ∣ succ₁ n
gcd-S≯S-∣₂ {m} {n} Nm Nn ih gcd-∣₁ Sm≯Sn =
  gcd-S≯S-∣₂-ah Nm Nn ih gcd-∣₁ Sm≯Sn
    (x∣y→x∣z→x∣y+z gcd-Sm,Sn-Sm-N Sn-Sm-N (nsucc Nm) ih gcd-∣₁)
    (x≤y→y∸x+x≡y (nsucc Nm) (nsucc Nn) (x≯y→x≤y (nsucc Nm) (nsucc Nn) Sm≯Sn))

  where
  Sn-Sm-N : N (succ₁ n ∸ succ₁ m)
  Sn-Sm-N = ∸-N (nsucc Nn) (nsucc Nm)

  gcd-Sm,Sn-Sm-N : N (gcd (succ₁ m) (succ₁ n ∸ succ₁ m))
  gcd-Sm,Sn-Sm-N = gcd-N (nsucc Nm) (Sn-Sm-N) (λ p → ⊥-elim (S≢0 (∧-proj₁ p)))

-- gcd (succ₁ m) (succ₁ n) ∣ succ₁ n when succ₁ m > succ₁ n.
postulate gcd-S>S-∣₂ : ∀ {m n} → N m → N n →
                       (gcd (succ₁ m ∸ succ₁ n) (succ₁ n) ∣ succ₁ n) →
                       succ₁ m > succ₁ n →
                       gcd (succ₁ m) (succ₁ n) ∣ succ₁ n
{-# ATP prove gcd-S>S-∣₂ #-}

------------------------------------------------------------------------------
-- The gcd is CD.
-- We will prove that gcdCD : ... → CD m n (gcd m n).

-- The gcd 0 (succ₁ n) is CD.
gcd-0S-CD : ∀ {n} → N n → CD zero (succ₁ n) (gcd zero (succ₁ n))
gcd-0S-CD Nn = (gcd-0S-∣₁ Nn , gcd-0S-∣₂ Nn)

-- The gcd (succ₁ m) 0 is CD.
gcd-S0-CD : ∀ {m} → N m → CD (succ₁ m) zero (gcd (succ₁ m) zero)
gcd-S0-CD Nm = (gcd-S0-∣₁ Nm , gcd-S0-∣₂ Nm)

-- The gcd (succ₁ m) (succ₁ n) when succ₁ m > succ₁ n is CD.
gcd-S>S-CD :
  ∀ {m n} → N m → N n →
  (CD (succ₁ m ∸ succ₁ n) (succ₁ n) (gcd (succ₁ m ∸ succ₁ n) (succ₁ n))) →
  succ₁ m > succ₁ n →
  CD (succ₁ m) (succ₁ n) (gcd (succ₁ m) (succ₁ n))
gcd-S>S-CD {m} {n} Nm Nn acc Sm>Sn =
   (gcd-S>S-∣₁ Nm Nn acc-∣₁ acc-∣₂ Sm>Sn , gcd-S>S-∣₂ Nm Nn acc-∣₂ Sm>Sn)
  where
  acc-∣₁ : gcd (succ₁ m ∸ succ₁ n) (succ₁ n) ∣ (succ₁ m ∸ succ₁ n)
  acc-∣₁ = ∧-proj₁ acc

  acc-∣₂ : gcd (succ₁ m ∸ succ₁ n) (succ₁ n) ∣ succ₁ n
  acc-∣₂ = ∧-proj₂ acc

-- The gcd (succ₁ m) (succ₁ n) when succ₁ m ≯ succ₁ n is CD.
gcd-S≯S-CD :
  ∀ {m n} → N m → N n →
  (CD (succ₁ m) (succ₁ n ∸ succ₁ m) (gcd (succ₁ m) (succ₁ n ∸ succ₁ m))) →
  succ₁ m ≯ succ₁ n →
  CD (succ₁ m) (succ₁ n) (gcd (succ₁ m) (succ₁ n))
gcd-S≯S-CD {m} {n} Nm Nn acc Sm≯Sn =
  (gcd-S≯S-∣₁ Nm Nn acc-∣₁ Sm≯Sn , gcd-S≯S-∣₂ Nm Nn acc-∣₂ acc-∣₁ Sm≯Sn)
  where
  acc-∣₁ : gcd (succ₁ m) (succ₁ n ∸ succ₁ m) ∣ succ₁ m
  acc-∣₁ = ∧-proj₁ acc

  acc-∣₂ : gcd (succ₁ m) (succ₁ n ∸ succ₁ m) ∣ (succ₁ n ∸ succ₁ m)
  acc-∣₂ = ∧-proj₂ acc

-- The gcd m n when m > n is CD.
gcd-x>y-CD :
  ∀ {m n} → N m → N n →
  (∀ {o p} → N o → N p → Lexi o p m n → x≢0≢y o p → CD o p (gcd o p)) →
  m > n →
  x≢0≢y m n →
  CD m n (gcd m n)
gcd-x>y-CD nzero          Nn             _  0>n   _ = ⊥-elim (0>x→⊥ Nn 0>n)
gcd-x>y-CD (nsucc Nm)     nzero          _  _     _ = gcd-S0-CD Nm
gcd-x>y-CD (nsucc {m} Nm) (nsucc {n} Nn) ah Sm>Sn _ =
  gcd-S>S-CD Nm Nn ih Sm>Sn
  where
  -- Inductive hypothesis.
  ih : CD (succ₁ m ∸ succ₁ n) (succ₁ n) (gcd (succ₁ m ∸ succ₁ n) (succ₁ n))
  ih  = ah {succ₁ m ∸ succ₁ n}
           {succ₁ n}
           (∸-N (nsucc Nm) (nsucc Nn))
           (nsucc Nn)
           ([Sx∸Sy,Sy]<[Sx,Sy] Nm Nn)
           (λ p → ⊥-elim (S≢0 (∧-proj₂ p)))

-- The gcd m n when m ≯ n is CD.
gcd-x≯y-CD :
  ∀ {m n} → N m → N n →
  (∀ {o p} → N o → N p → Lexi o p m n → x≢0≢y o p → CD o p (gcd o p)) →
  m ≯ n →
  x≢0≢y m n →
  CD m n (gcd m n)
gcd-x≯y-CD nzero          nzero         _   _     h = ⊥-elim (h (refl , refl))
gcd-x≯y-CD nzero          (nsucc Nn)     _  _     _ = gcd-0S-CD Nn
gcd-x≯y-CD (nsucc _)      nzero          _  Sm≯0  _ = ⊥-elim (S≯0→⊥ Sm≯0)
gcd-x≯y-CD (nsucc {m} Nm) (nsucc {n} Nn) ah Sm≯Sn _ = gcd-S≯S-CD Nm Nn ih Sm≯Sn
  where
  -- Inductive hypothesis.
  ih : CD (succ₁ m) (succ₁ n ∸ succ₁ m)  (gcd (succ₁ m) (succ₁ n ∸ succ₁ m))
  ih = ah {succ₁ m}
          {succ₁ n ∸ succ₁ m}
          (nsucc Nm)
          (∸-N (nsucc Nn) (nsucc Nm))
          ([Sx,Sy∸Sx]<[Sx,Sy] Nm Nn)
          (λ p → ⊥-elim (S≢0 (∧-proj₁ p)))

-- The gcd is CD.
gcdCD : ∀ {m n} → N m → N n → x≢0≢y m n → CD m n (gcd m n)
gcdCD = Lexi-wfind A h
  where
  A : D → D → Set
  A i j = x≢0≢y i j → CD i j (gcd i j)

  h : ∀ {i j} → N i → N j → (∀ {k l} → N k → N l → Lexi k l i j → A k l) →
      A i j
  h Ni Nj ah = case (gcd-x>y-CD Ni Nj ah) (gcd-x≯y-CD Ni Nj ah) (x>y∨x≯y Ni Nj)
